paxos/network.dfy
@@ -1,13 +1,36 @@
+include "types.dfy"
+
 module Network {
+import opened Types
 
-datatype Packet<IdType, MessageType> = Packet(src:IdType, dst:IdType, msg:MessageType)
+datatype EnvStep = 
+    IoStep(actor:Id, recvIos:seq<Packet>, sendIos:seq<Packet>)
 
-datatype EnvStep<IdType, MessageType> = 
-    IoStep(actor:IdType, recvIo:Packet<IdType, MessageType>, sendIos:seq<Packet<IdType, MessageType>>)
-
-datatype Environment<IdType(==), MessageType(==)> = Env(
-        sentPackets:set<Packet<IdType, MessageType>>,
-        recvdPackets:set<Packet<IdType, MessageType>>,
-        nextStep:EnvStep<IdType, MessageType>
+datatype Environment = Env(
+        sentPackets:set<Packet>,
+        nextStep:EnvStep
     )
+
+predicate EnvironmentInit(e:Environment) {
+    e.sentPackets == {}
+}
+
+predicate ValidIoStep(iostep:EnvStep) 
+    requires iostep.IoStep?
+{
+    && (forall r | r in iostep.recvIos :: r.dst == iostep.actor)
+    && (forall s | s in iostep.sendIos :: s.src == iostep.actor)
+}
+
+
+predicate EnvironmentNext(e:Environment, e':Environment)
+{
+    match e.nextStep {
+        case IoStep(actor, recvIos, sendIos) => 
+            && ValidIoStep(e.nextStep)
+            && e'.sentPackets == e.sentPackets + (set s | s in sendIos)
+            && (forall r | r in recvIos :: r in e.sentPackets)
+    }
+}
+
 }
