paxos/synod.dfy
@@ -1,19 +1,79 @@
+include "types.dfy"
 include "network.dfy"
 include "agents.dfy"
 
 module Synod {
 import opened Network
 import opened Agents
+import opened Types
 
 
 datatype DistrSys = DistrSys(
-    network: Environment<Id, Message>,
-    leaders: seq<Leader<Id, Ballot, Value>>,
-    acceptors: seq<Acceptor<Ballot, Value>>
+    network: Environment,
+    leaders: seq<Leader>,
+    acceptors: seq<Acceptor>
 )
 
-datatype Step = PaxosStep(src:Id)
+
+/*****************************************************************************************
+*                                        DS Init                                         *
+*****************************************************************************************/
+predicate Init(s:DistrSys, f:nat, l:nat, accConf:seq<Id>) 
+    requires f >= 1;
+    requires l >= 1;
+    requires ValidAccConf(f, accConf)
+{
+    && EnvironmentInit(s.network)
+    && |s.leaders| == l
+    && (forall i | 0 <= i < l :: LeaderInit(s.leaders[i], Id(Ldr, i), accConf, f, V(i)))
+    && |s.acceptors| == 2*f+1
+    && (forall i | 0 <= i < 2*f+1 :: AcceptorInit(s.acceptors[i], accConf[i]))
+}
+
+predicate ValidAccConf(f:nat, accConf:seq<Id>) {
+    && |accConf| == 2*f+1
+    && (forall i | 0 <= i < |accConf| :: accConf[i] == Id(Acc, i))
+}
+
+// predicate AccConfUnique(accConf:seq<Id>) {
+//     forall i,j | 0 <= i < |accConf| && 0 <= j < |accConf| 
+//     :: accConf[i].idx == accConf[j].idx ==> i == j
+// }
 
 
+/*****************************************************************************************
+*                                        DS Next                                         *
+*****************************************************************************************/
 
+predicate PaxosNextOneAgent(s:DistrSys, s':DistrSys, src:Id, recvIos:seq<Packet>, sendIos:seq<Packet>) 
+{
+    && ValidSrc(s, src)
+    && PaxosNextOneAgent_Agent(s, s', src, recvIos, sendIos)
+    && s.network.nextStep == IoStep(src, recvIos, sendIos)
+    && EnvironmentNext(s.network, s'.network)
+}
+
+predicate PaxosNextOneAgent_Agent(s:DistrSys, s':DistrSys, src:Id, recvIos:seq<Packet>, sendIos:seq<Packet>)
+    requires ValidSrc(s, src)
+{
+    match src.agt {
+        case Ldr() => 
+            && s'.acceptors == s.acceptors
+            && |s'.leaders| == |s.leaders|
+            && s'.leaders == s.leaders[src.idx := s'.leaders[src.idx]]
+            && LeaderNext(s.leaders[src.idx], s'.leaders[src.idx], recvIos, sendIos)
+        case Acc() => 
+            && s'.leaders == s.leaders
+            && |s'.acceptors| == |s.acceptors|
+            && s'.acceptors == s.acceptors[src.idx := s'.acceptors[src.idx]]
+            && AcceptorNext(s.acceptors[src.idx], s'.acceptors[src.idx], recvIos, sendIos)
+    }
+}
+
+predicate ValidSrc(s:DistrSys, src:Id) {
+     match src.agt {
+        case Ldr() => 0 <= src.idx < |s.leaders|
+        case Acc() => 0 <= src.idx < |s.acceptors|
+    }
+}
 }
